

$$\textcircled{1} a) |\psi\rangle = \begin{pmatrix} \alpha_1 \\ \beta_1 \end{pmatrix} \otimes \begin{pmatrix} \alpha_2 \\ \beta_2 \end{pmatrix} = \begin{pmatrix} \alpha_1 \alpha_2 \\ \alpha_1 \beta_2 \\ \beta_1 \alpha_2 \\ \beta_1 \beta_2 \end{pmatrix}$$

$$\hat{S}^2 = (\hat{S}_1 + \hat{S}_2)^2 = \hat{S}_1^2 + \hat{S}_2^2 + 2\hat{S}_1 \cdot \hat{S}_2$$

$$\hat{S}_1^2 = \hat{S}_2^2 = \frac{3}{4} \hbar^2 \begin{pmatrix} 1 & 0 \\ 0 & 1 \end{pmatrix} = \frac{3}{4} \hbar^2 \mathbb{1}^{2 \times 2}$$

$$\text{To be fully precise: } \hat{S}^2 = (\hat{S}_1 \otimes \mathbb{1}_2 + \hat{S}_2 \otimes \mathbb{1}_1)^2$$

$$= \hat{S}_1^2 \otimes \mathbb{1}_2^2 + \mathbb{1}_1^2 \otimes \hat{S}_2^2 + 2\hat{S}_1 \otimes \hat{S}_2$$

$$\frac{3}{4} \hbar^2 \mathbb{1}^{2 \times 2} \otimes \mathbb{1}^{2 \times 2} = \frac{3}{4} \hbar^2 \mathbb{1}^{4 \times 4}$$

$$2(\hat{S}_{1,x} \otimes \hat{S}_{2,x} + \hat{S}_{1,y} \otimes \hat{S}_{2,y} + \hat{S}_{1,z} \otimes \hat{S}_{2,z})$$

$$= \hat{S}_{1,+} \otimes \hat{S}_{2,-} + \hat{S}_{1,-} \otimes \hat{S}_{2,+} + 2\hat{S}_{1,z} \otimes \hat{S}_{2,z}$$

$$\left. \begin{aligned} \hat{S}_+ &= \hat{S}_x + i\hat{S}_y \\ \hat{S}_- &= \hat{S}_x - i\hat{S}_y \end{aligned} \right\} \Rightarrow \begin{aligned} \hat{S}_x &= \frac{1}{2}(\hat{S}_+ + \hat{S}_-) \\ \hat{S}_y &= \frac{1}{2i}(\hat{S}_+ - \hat{S}_-) \end{aligned}$$

$$\hookrightarrow \hat{S}_{1,x} \otimes \hat{S}_{2,x} = \frac{1}{4}(\hat{S}_{1,+} \otimes \hat{S}_{2,+} + \hat{S}_{1,-} \otimes \hat{S}_{2,-} + \hat{S}_{1,-} \otimes \hat{S}_{2,+} + \hat{S}_{1,+} \otimes \hat{S}_{2,-})$$

$$\hat{S}_{1,y} \otimes \hat{S}_{2,y} = -\frac{1}{4}(\hat{S}_{1,+} \otimes \hat{S}_{2,-} - \hat{S}_{1,-} \otimes \hat{S}_{2,+} - \hat{S}_{1,-} \otimes \hat{S}_{2,-} + \hat{S}_{1,+} \otimes \hat{S}_{2,+})$$

$$\hookrightarrow \hat{S}_{1,x} \otimes \hat{S}_{2,x} + \hat{S}_{1,y} \otimes \hat{S}_{2,y} = \frac{1}{2}(\hat{S}_{1,+} \otimes \hat{S}_{2,-} + \hat{S}_{1,-} \otimes \hat{S}_{2,+})$$

$$\Rightarrow \hat{S}^2 = 2 \cdot \frac{3}{4} \hbar^2 \mathbb{1}^{4 \times 4} + \hbar^2 \left[\underbrace{\begin{pmatrix} 0 & 1 \\ 0 & 0 \end{pmatrix} \otimes \begin{pmatrix} 0 & 0 \\ 1 & 0 \end{pmatrix}}_{\begin{pmatrix} 0 & 0 & 0 & 0 \\ 0 & 1 & 1 & 0 \\ 0 & 1 & 1 & 0 \\ 0 & 0 & 0 & 2 \end{pmatrix}} + \underbrace{\begin{pmatrix} 0 & 0 \\ 1 & 0 \end{pmatrix} \otimes \begin{pmatrix} 0 & 1 \\ 0 & 0 \end{pmatrix}}_{\begin{pmatrix} 0 & 0 & 0 & 0 \\ 0 & 1 & 1 & 0 \\ 0 & 1 & 1 & 0 \\ 0 & 0 & 0 & 2 \end{pmatrix}} + \frac{1}{2} \underbrace{\begin{pmatrix} 1 & 0 & 0 & 0 \\ 0 & -1 & 0 & 0 \\ 0 & 0 & 1 & 0 \\ 0 & 0 & 0 & -1 \end{pmatrix}}_{\begin{pmatrix} 1 & 0 & 0 & 0 \\ 0 & -1 & 0 & 0 \\ 0 & 0 & 1 & 0 \\ 0 & 0 & 0 & -1 \end{pmatrix}} \right]$$

$$= \hbar^2 \begin{pmatrix} 2 & 0 & 0 & 0 \\ 0 & 1 & 1 & 0 \\ 0 & 1 & 1 & 0 \\ 0 & 0 & 0 & 2 \end{pmatrix}$$

b) 2 el. sp., since sp. has off-diagonals

c) Edges are already decoupled and inner 2x2 is diagonalized by equal lin. combs, so eigenpairs are $2\hbar^2 : (\uparrow\uparrow)$, $2\hbar^2 : (\uparrow\downarrow + \downarrow\uparrow)$, $0 : (\uparrow\downarrow - \downarrow\uparrow)$, $2\hbar^2 : (\downarrow\downarrow)$

e) + d) States 1, 2 and 4 are triplets ($S=1$) with $M_S = 1, 0, -1$, respectively and state 3 is a singlet with $S=0$ and $M_S=0$, uniquely characterizing the eigenfunctions

① a) $\chi_1 = \phi_5 \alpha$ $\chi_2 = \phi_{11} \alpha$

$$\Rightarrow |\chi\rangle = |\chi_1 \chi_2\rangle = \phi_5^1 \alpha^1 \phi_{11}^2 \alpha^2 - \phi_{11}^1 \alpha^1 \phi_5^2 \alpha^2$$

$$= \alpha_1 \alpha_2 (\phi_5^1 \phi_{11}^2 - \phi_{11}^1 \phi_5^2)$$

b) $\hat{J}^2 = \hat{J}_x^2 + \hat{J}_y^2 + \hat{J}_z^2 = \hat{J}_z^2 + \hbar \hat{J}_z + \hat{J}_- \hat{J}_+$

$$\hookrightarrow \hat{J}_x^2 + \hat{J}_y^2 = \hbar \hat{J}_z + \hat{J}_- \hat{J}_+ = \hbar \hat{J}_z + \hat{J}_x^2 + \hat{J}_y^2 + \underbrace{i[\hat{J}_x, \hat{J}_y]}_{= \hbar \hat{J}_z} = -\hbar \hat{J}_z$$

$$= i\hbar \hat{J}_z$$

c) $\hat{J}_z (\hat{L}_z + \hat{S}_z) |\chi\rangle = 2\hbar |\chi\rangle$

$$\hookrightarrow \hat{S}_z |\alpha_1 \alpha_2\rangle = \hbar$$

$$\hookrightarrow \hat{L}_z |\phi_5^1 \phi_{11}^2\rangle = (\hat{L}_{z1} + \hat{L}_{z2}) |\phi_5^1 \phi_{11}^2\rangle = \underbrace{\hat{L}_{z1} |\phi_5^1\rangle}_{=0} + \underbrace{\hat{L}_{z2} |\phi_{11}^2\rangle}_{=\hbar} = \hbar$$

d) $\hat{J}^2 |\chi\rangle = [\hat{J}_z^2 + \hbar \hat{J}_z + \hat{J}_- \hat{J}_+] |\chi\rangle$

$$\Rightarrow \hbar \hat{J}_z |\chi\rangle = 2\hbar^2 |\chi\rangle$$

$$\Rightarrow \hat{J}_z^2 |\chi\rangle = 4\hbar^2 |\chi\rangle$$

$\Rightarrow \hat{J}_- \hat{J}_+ |\chi\rangle = 0$, because $\hat{J}_+ |\chi\rangle = 0$, because 1 and 1 can't be linearly combined to something higher than 2, which is the eigenvalue of $|\chi\rangle$

e) $2s+1 L_J \rightarrow {}^3P_2$